introduce NeverHeldInvariant with proof sketch of PerformanceGuaranteeHolds_Induction_IOStep

ironfleet/src/Dafny/Distributed/Protocol/Lock/PerformanceProof/EmptyPerformanceProof.i.dfy
@@ -24,6 +24,7 @@ predicate PerformanceInductiveInvariant(config:ConcreteConfiguration, tgls:Times
     && HistoryLengthInvariant(config, tgls)
     && TransferInvariant(tgls)
     && LockedInvariant(tgls)
+    && NeverHeldInvariant(tgls)
 }
 
 
@@ -31,9 +32,9 @@ predicate TransferInvariant(tgls:TimestampedGLS_State) {
     forall pkt  
         | && pkt in tgls.tls.t_environment.sentPackets 
           && pkt.msg.v.Transfer?
-        :: 0 < pkt.msg.v.transfer_epoch <= |tgls.tls.config|
-           ==> 
-           TimeEq(pkt.msg.ts, PerfBoundLockInNetwork(pkt.msg.v.transfer_epoch))
+          && 0 < pkt.msg.v.transfer_epoch <= |tgls.tls.config|  // first round 
+        ::
+          TimeEq(pkt.msg.ts, PerfBoundLockInNetwork(pkt.msg.v.transfer_epoch))
 } 
 
 
@@ -41,10 +42,19 @@ predicate LockedInvariant(tgls:TimestampedGLS_State) {
     forall ep 
         | && ep in tgls.tls.t_servers
           && tgls.tls.t_servers[ep].v.held
-        :: 0 < tgls.tls.t_servers[ep].v.epoch <= |tgls.tls.config|
-           ==> 
-           TimeEq(tgls.tls.t_servers[ep].ts, PerfBoundLockHeld(tgls.tls.t_servers[ep].v.epoch))
+          && 0 < tgls.tls.t_servers[ep].v.epoch <= |tgls.tls.config|  // first round
+        ::
+          TimeEq(tgls.tls.t_servers[ep].ts, PerfBoundLockHeld(tgls.tls.t_servers[ep].v.epoch))
 } 
+
+
+predicate NeverHeldInvariant(tgls:TimestampedGLS_State) {
+    forall ep 
+        | && ep in tgls.tls.t_servers
+          && tgls.tls.t_servers[ep].v.epoch == 0 
+        ::
+          TimeEq(tgls.tls.t_servers[ep].ts, TimeZero());
+}
 
 
 
@@ -137,37 +147,103 @@ lemma PerformanceGuaranteeHolds_Induction_IOStep(config:Config, tgls:Timestamped
     ensures PerformanceInductiveInvariant(config, tgls');
 {
     var tls, tls' := tgls.tls, tgls'.tls;
-    var e, e' := tls.t_environment, tls'.t_environment;
-    var id, ios, hstep := e.nextStep.actor, e.nextStep.ios, e.nextStep.nodeStep;
+    var id, ios, hstep := tls.t_environment.nextStep.actor, tls.t_environment.nextStep.ios, tls.t_environment.nextStep.nodeStep;
 
     assert TLS_NextOneServer(tls, tls', id, ios, hstep);
     if |ios| > 0 && ios[0].LIoOpReceive? {
-        // NodeAccept branch
-        assert tls'.t_servers[id].ts == TLS_RecvPerfUpdate(tls.t_servers[id].ts, ios[0].r.msg.ts, hstep);
-        assert hstep == AcceptStep;
-        var ls, ls', untagged_ios := UntagLS_State(tls), UntagLS_State(tls'), UntagLIoOpSeq(ios);
-        assert NodeAccept(ls.servers[id], ls'.servers[id], untagged_ios);
-        if !ls.servers[id].held 
-           && untagged_ios[0].r.src in ls.servers[id].config
-           && untagged_ios[0].r.msg.Transfer? 
-           && untagged_ios[0].r.msg.transfer_epoch > ls.servers[id].epoch 
-        {
-            // TODO
-            assume false;
-        } else {
-            /* This branch cannot occur, because it means that the node is either 
-            * processing a locked message, or a non-in-flight transfer message. Both can
-            * only occur after the node has received the lock for the first time */
-
-            assume false;
-        }
+        PerformanceGuaranteeHolds_Induction_IOStep_Accept(config, tgls, tgls');
     } else {
-        // NodeGrant branch
-        assert tls'.t_servers[id].ts == TLS_NoRecvPerfUpdate(tls.t_servers[id].ts, hstep);
-        assume false;
+        PerformanceGuaranteeHolds_Induction_IOStep_Grant(config, tgls, tgls');
     }
     assert TransferInvariant(tgls');
     assert LockedInvariant(tgls');
+}
+
+
+lemma PerformanceGuaranteeHolds_Induction_IOStep_Accept(config:Config, tgls:TimestampedGLS_State, tgls':TimestampedGLS_State)
+    // Standard pre-conditions
+    requires |tgls.history| > 0 && |tgls'.history| > 0;
+    requires PerformanceInductiveInvariant(config, tgls);
+    requires ConfigInvariant(config, tgls');
+    requires HistoryLengthInvariant(config, tgls');
+    requires SingleGLSPerformanceAssumption(tgls) && SingleGLSPerformanceAssumption(tgls');
+    requires TGLS_Next(tgls, tgls');
+    // Branch condition
+    requires tgls.tls.t_environment.nextStep.LEnvStepHostIos? && tgls.tls.t_environment.nextStep.actor in tgls.tls.t_servers;
+    requires |tls.t_environment.nextStep.ios| > 0 && tls.t_environment.nextStep.ios[0].LIoOpReceive?
+    // Post-conditions
+    ensures PerformanceInductiveInvariant(config, tgls');
+{
+    var tls, tls' := tgls.tls, tgls'.tls;
+    var e, e' := tls.t_environment, tls'.t_environment;
+    var id, ios, hstep := e.nextStep.actor, e.nextStep.ios, e.nextStep.nodeStep;
+    assert TLS_NextOneServer(tls, tls', id, ios, hstep);
+
+    assert tls'.t_servers[id].ts == TLS_RecvPerfUpdate(tls.t_servers[id].ts, ios[0].r.msg.ts, hstep);
+    assert hstep == AcceptStep;
+    var ls, ls', untagged_ios := UntagLS_State(tls), UntagLS_State(tls'), UntagLIoOpSeq(ios);
+    assert NodeAccept(ls.servers[id], ls'.servers[id], untagged_ios);
+    if !ls.servers[id].held 
+        && untagged_ios[0].r.src in ls.servers[id].config
+        && untagged_ios[0].r.msg.Transfer? 
+        && untagged_ios[0].r.msg.transfer_epoch > ls.servers[id].epoch 
+    {
+        /* I do not hold the lock. Hence, the updated counter is the max of the 
+        * message counter and my local counter. The message counter has the desired 
+        * counter by TransferInvariant. If my local epoch is 0, then my local counter
+        * is 0 by NeverHeldInvariant, and I get the desired local update that 
+        * satisfies LockedInvariant.
+        * If my local epoch is x != 0, Then my epoch must by x + n|config| for n >= 0. 
+        * (LEMMA) Then LockedInvariant is trivially satisfied. */ 
+        assume false;
+    } else {
+        /* By assumption, I do not hold lock. Hence, TransferInvariant and 
+        * LockedInvariant are trivially satisfied for the next step because I am not 
+        * emitting any Transfer packets, nor am I going to hold the lock. Hence, I 
+        * am tasked with satisfying NeverHeldInvariant in the next step.
+        * If my ep != 0, invariant is trivially satisfied.
+        * Else, if receiving a Transfer message, any Transfer message destined for me 
+        * must be in flight, so contradiction (LEMMA). I could also be receiving a 
+        * Locked message. In this case my epoch cannot be 0 (LEMMA), 
+        * so contradiction again. */
+        assume false;
+    }
+}
+
+
+lemma PerformanceGuaranteeHolds_Induction_IOStep_Grant(config:Config, tgls:TimestampedGLS_State, tgls':TimestampedGLS_State)
+    // Standard pre-conditions
+    requires |tgls.history| > 0 && |tgls'.history| > 0;
+    requires PerformanceInductiveInvariant(config, tgls);
+    requires ConfigInvariant(config, tgls');
+    requires HistoryLengthInvariant(config, tgls');
+    requires SingleGLSPerformanceAssumption(tgls) && SingleGLSPerformanceAssumption(tgls');
+    requires TGLS_Next(tgls, tgls');
+    // Branch condition
+    requires tgls.tls.t_environment.nextStep.LEnvStepHostIos? && tgls.tls.t_environment.nextStep.actor in tgls.tls.t_servers;
+    requires !(|tls.t_environment.nextStep.ios| > 0 && tls.t_environment.nextStep.ios[0].LIoOpReceive?)
+    // Post-conditions
+    ensures PerformanceInductiveInvariant(config, tgls');
+{
+    var tls, tls' := tgls.tls, tgls'.tls;
+    var e, e' := tls.t_environment, tls'.t_environment;
+    var id, ios, hstep := e.nextStep.actor, e.nextStep.ios, e.nextStep.nodeStep;
+    assert TLS_NextOneServer(tls, tls', id, ios, hstep);
+
+    assert tls'.t_servers[id].ts == TLS_NoRecvPerfUpdate(tls.t_servers[id].ts, hstep);
+    assert hstep == GrantStep;
+    var ls, ls', untagged_ios := UntagLS_State(tls), UntagLS_State(tls'), UntagLIoOpSeq(ios);
+    assert NodeGrant(ls.servers[id], ls'.servers[id], untagged_ios);
+    if ls.servers[id].held && ls.servers[id].epoch < 0xFFFF_FFFF_FFFF_FFFF {
+        /* Locked invariant easily implies Transfer invariant in the next step.
+        * ep != 0, so NeverHeldInvariant trivially satisfied. */
+        assume false;
+    } else {
+        /* If my epoch >= 0xFFFF_FFFF_FFFF_FFFF, by HistoryLengthInvariant, |history|
+        * >= 0xFFFF_FFFF_FFFF_FFFF, violating SingleGLSPerformanceAssumption.
+        * Else, I don't hold lock. This violates SingleGLSPerformanceAssumption. */
+        assume false;
+    }
 }
 
 
